theories/Data/FiniteSet.v
@@ -1,4 +1,5 @@
 Require Import PnV.Prelude.Prelude.
+Require Import PnV.Prelude.X.
 
 #[local] Infix "=~=" := is_similar_to : type_scope.
 #[local] Infix "\in" := E.In.
